src/ops/insert.v
@@ -1,0 +1,27 @@
+From Ssreflect
+     Require Import ssreflect ssrbool eqtype ssrnat seq fintype ssrfun.
+From MathComp
+     Require Import tuple finset.
+From Bits
+     Require Import bits.
+Require Import props.getbit spec.
+
+Definition insert {n}(bs: BITS n) k: BITS n
+  := orB bs (shlBn #1 k).
+
+Lemma insert_repr:
+  forall n (bs: BITS n) (k: 'I_n) E, repr bs E ->
+    repr (insert bs k) (k |: E).
+Proof.
+  move=> n bs k E HE.
+  rewrite /repr -setP /eq_mem=> x.
+  rewrite in_set getBit_set_true=> //.
+  rewrite fun_if.
+  case H: (x == k).
+    + (* Case: x == k *)
+      move/eqP: H ->.
+      by rewrite eq_refl setU11.
+    + (* Case: x <> k *)
+      rewrite ifF=> //.
+      by rewrite in_setU1 H HE in_set.
+Qed.
